LambdaLab.lean
@@ -55,7 +55,7 @@ import LambdaLab.Abstraction.Tokenizer
 import LambdaLab.Arith.Pipeline
 import LambdaLab.Inductive.Basic
 import LambdaLab.Inductive.Example
-import LambdaLab.Nominal.Basic
+import LambdaLab.Nominal.Atom
 import LambdaLab.TypeSystem.Named.Context
 import LambdaLab.TypeSystem.Named.Basic
 import LambdaLab.TypeSystem.Intrinsic.Basic
